@prefix : <http://www.semanticweb.org/radmehr/ontologies/2024/9/untitled-ontology-36/> .
@prefix owl: <http://www.w3.org/2002/07/owl#> .
@prefix rdf: <http://www.w3.org/1999/02/22-rdf-syntax-ns#> .
@prefix xml: <http://www.w3.org/XML/1998/namespace> .
@prefix xsd: <http://www.w3.org/2001/XMLSchema#> .
@prefix rdfs: <http://www.w3.org/2000/01/rdf-schema#> .
@base <http://www.semanticweb.org/radmehr/ontologies/2024/9/untitled-ontology-36/> .

<https://w3id.org/FAIR-course-UT/2024-2025/10/ont#> rdf:type owl:Ontology ;
                                                     owl:versionIRI <https://w3id.org/FAIR-course-UT/2024-2025/10/ont#> .

#################################################################
#    Object Properties
#################################################################

###  http://www.semanticweb.org/radmehr/ontologies/2024/9/untitled-ontology-36/contains
:contains rdf:type owl:ObjectProperty ;
          rdfs:domain :Air_pollution_measurement ;
          rdfs:range :Pollutant ;
          rdfs:comment "The predicate that relates Domain: (blank)_Cell to Range: Pollutant, indicating that the (blank)_Cell as a nested node containts Pollutant (pollutant type)" ;
          rdfs:label "contains" .


###  http://www.semanticweb.org/radmehr/ontologies/2024/9/untitled-ontology-36/hasCode
:hasCode rdf:type owl:ObjectProperty ;
         rdfs:domain :Country ;
         rdfs:range :Country_Code ;
         rdfs:comment "The predicate that relates Domain: Country Lable to Range: Country Code, indicating that the Country Lable hasCode Country Code (i.e. Germany hasCode DE)" ;
         rdfs:label "hasCode" .


###  http://www.semanticweb.org/radmehr/ontologies/2024/9/untitled-ontology-36/hasSource
:hasSource rdf:type owl:ObjectProperty ;
           rdfs:domain :Air_Quality_Monitoring ;
           rdfs:range :Source_Name ;
           rdfs:comment "The predicate that relates Domain: particulate matter air pollution measurement to Range: Source Name, indicating that the particulate matter air pollution measurement measurements are comin from which Source" ;
           rdfs:label "hasSource" .


###  http://www.semanticweb.org/radmehr/ontologies/2024/9/untitled-ontology-36/hasUnit
:hasUnit rdf:type owl:ObjectProperty ;
         rdfs:domain :Air_pollution_measurement ;
         rdfs:range :Unit ;
         rdfs:comment "The predicate that relates Domain:(blank)_Cell to Range:Unit, indicating that the (blank)_Cell as a nested node hasUnit Unit" ;
         rdfs:label "hasUnit" .


###  http://www.semanticweb.org/radmehr/ontologies/2024/9/untitled-ontology-36/locatedIn
:locatedIn rdf:type owl:ObjectProperty ;
           rdfs:domain :City ;
           rdfs:range :Country ;
           rdfs:comment "The predicate that relates Domain: City to Range: Counry Label, indicating that the City is locatedIn Country Label" ;
           rdfs:label "locatedIn" .


###  http://www.semanticweb.org/radmehr/ontologies/2024/9/untitled-ontology-36/measures
:measures rdf:type owl:ObjectProperty ;
          rdfs:domain :Air_Quality_Monitoring ;
          rdfs:range :Air_pollution_measurement ;
          rdfs:comment "The predicate that relates Domain:particulate matter air pollution measurement to Range:(blank)_Cell, indicating that the particulate matter air pollution measurement mesures the nested node (blank)_Cell" ;
          rdfs:label "measures" .


###  http://www.semanticweb.org/radmehr/ontologies/2024/9/untitled-ontology-36/occursIn
:occursIn rdf:type owl:ObjectProperty ;
          rdfs:domain :Air_Quality_Monitoring ;
          rdfs:range :Location ;
          rdfs:comment "The predicate that relates Domain:particulate matter air pollution measurement to Range:Location, indicating that the particulate matter air pollution measurement occurs in the Location" ;
          rdfs:label "occursIn" .


###  https://w3id.org/FAIR-course-UT/2024-2025/10/ont#hasCity
:hasCity rdf:type owl:ObjectProperty ;
         rdfs:domain :Location ;
         rdfs:range :City ;
         rdfs:comment "The predicate that relates Domain:Location to Range:City, indicating that the Location is locatedIn City" .


#################################################################
#    Data properties
#################################################################

###  http://www.semanticweb.org/radmehr/ontologies/2024/9/untitled-ontology-36/hasCoordination
:hasCoordination rdf:type owl:DatatypeProperty ;
                 rdfs:domain :Location ;
                 rdfs:range xsd:decimal ;
                 rdfs:comment "Indicates the Coordinates in type decimal" ;
                 rdfs:label "hasCoordination" .


###  http://www.semanticweb.org/radmehr/ontologies/2024/9/untitled-ontology-36/hasValue
:hasValue rdf:type owl:DatatypeProperty ;
          rdfs:domain :Air_pollution_measurement ;
          rdfs:range xsd:decimal .


###  https://w3id.org/FAIR-course-UT/2024-2025/10/ont#dateModified
:dateModified rdf:type owl:DatatypeProperty ;
              rdfs:domain :Air_Quality_Monitoring ;
              rdfs:range xsd:dateTimeStamp ;
              rdfs:comment "Date on which the resource was changed." ;
              rdfs:label "dateModified" .


#################################################################
#    Classes
#################################################################

###  http://www.semanticweb.org/radmehr/ontologies/2024/9/untitled-ontology-36/Air_Quality_Monitoring
:Air_Quality_Monitoring rdf:type owl:Class ;
                        rdfs:comment "OpenAQ Air Quality Monitoring: An open, real-time air quality data hub for the world" ;
                        rdfs:label "Air Quality Monitoring" .


###  http://www.semanticweb.org/radmehr/ontologies/2024/9/untitled-ontology-36/Air_pollution_measurement
:Air_pollution_measurement rdf:type owl:Class ;
                           rdfs:comment "Process of collecting and measuring the components of air pollution" ;
                           rdfs:label "Air pollution measurement" .


###  http://www.semanticweb.org/radmehr/ontologies/2024/9/untitled-ontology-36/City
:City rdf:type owl:Class ;
      rdfs:comment "The city or town associated with the address of the object. cf. vcard:locality" ;
      rdfs:label "City" .


###  http://www.semanticweb.org/radmehr/ontologies/2024/9/untitled-ontology-36/Country
:Country rdf:type owl:Class ;
         rdfs:comment "The name of the country or major administrative unit in which the Location occurs." ;
         rdfs:label "Country" .


###  http://www.semanticweb.org/radmehr/ontologies/2024/9/untitled-ontology-36/Country_Code
:Country_Code rdf:type owl:Class ;
              rdfs:comment "An alphanumeric system designed to identify countries. The ISO 3166 standard includes a two letter representation, a three letter representation, and a 3 number representation. The last two are identical to the UN system. The US State Department system maintains a separate two letter representation code set." ;
              rdfs:label "Country Code" .


###  http://www.semanticweb.org/radmehr/ontologies/2024/9/untitled-ontology-36/Location
:Location rdf:type owl:Class ;
          rdfs:comment "Representing a named geographical place" ;
          rdfs:label "Location" .


###  http://www.semanticweb.org/radmehr/ontologies/2024/9/untitled-ontology-36/Pollutant
:Pollutant rdf:type owl:Class ;
           rdfs:comment "Any chemical compound, biological object, physical factor in a concentration or amount that adversely alters the physical, chemical, or biological properties of the environment. The term includes pathogens, toxic metals, carcinogens, oxygen-demanding materials, radiation, natural substances, synthetic industrial chemicals, biocides and all other harmful substances and factors. (NCI)" ;
           rdfs:label "Pollutant" .


###  http://www.semanticweb.org/radmehr/ontologies/2024/9/untitled-ontology-36/Source_Name
:Source_Name rdf:type owl:Class ;
             rdfs:comment "The name of the center or institution that provided an item." ;
             rdfs:label "Source Name" .


###  http://www.semanticweb.org/radmehr/ontologies/2024/9/untitled-ontology-36/Unit
:Unit rdf:type owl:Class ;
      rdfs:comment "A unit of measurement is a definite magnitude of a physical quantity, defined and adopted by convention and/or by law, that is used as a standard for measurement of the same physical quantity." ;
      rdfs:label "Unit" .


#################################################################
#    Individuals
#################################################################

###  http://www.semanticweb.org/radmehr/ontologies/2024/9/untitled-ontology-36/Airgradient
:Airgradient rdf:type owl:NamedIndividual ,
                      :Source_Name ;
             rdfs:comment "An instanse of class Source Name" ;
             rdfs:label "Airgradient" .


###  http://www.semanticweb.org/radmehr/ontologies/2024/9/untitled-ontology-36/CO
:CO rdf:type owl:NamedIndividual ,
             :Pollutant ;
    rdfs:comment "An instance of class Pollutant" ;
    rdfs:label "CO" .


###  http://www.semanticweb.org/radmehr/ontologies/2024/9/untitled-ontology-36/EEA
:EEA rdf:type owl:NamedIndividual ,
              :Source_Name ;
     rdfs:comment "An instance of class Source Name" ;
     rdfs:label "EEA" .


###  http://www.semanticweb.org/radmehr/ontologies/2024/9/untitled-ontology-36/EEA_France
:EEA_France rdf:type owl:NamedIndividual ,
                     :Source_Name ;
            rdfs:comment "An instance of class Source Name" ;
            rdfs:label "EEA France" .


###  http://www.semanticweb.org/radmehr/ontologies/2024/9/untitled-ontology-36/EEA_Germany
:EEA_Germany rdf:type owl:NamedIndividual ,
                      :Source_Name ;
             rdfs:comment "An instance of class Source Name" ;
             rdfs:label "EEA Germany" .


###  http://www.semanticweb.org/radmehr/ontologies/2024/9/untitled-ontology-36/GIOS
:GIOS rdf:type owl:NamedIndividual ,
               :Source_Name ;
      rdfs:comment "An instance of class Source Name" ;
      rdfs:label "GIOS" .


###  http://www.semanticweb.org/radmehr/ontologies/2024/9/untitled-ontology-36/NO
:NO rdf:type owl:NamedIndividual ,
             :Pollutant ;
    rdfs:comment "An instance of class Pollutant" ;
    rdfs:label "NO" .


###  http://www.semanticweb.org/radmehr/ontologies/2024/9/untitled-ontology-36/NO2
:NO2 rdf:type owl:NamedIndividual ,
              :Pollutant ;
     rdfs:comment "An instance of class Pollutant" ;
     rdfs:label "NO2" .


###  http://www.semanticweb.org/radmehr/ontologies/2024/9/untitled-ontology-36/O3
:O3 rdf:type owl:NamedIndividual ,
             :Pollutant ;
    rdfs:comment "An instance of class Pollutant" ;
    rdfs:label "O3" .


###  http://www.semanticweb.org/radmehr/ontologies/2024/9/untitled-ontology-36/PM1
:PM1 rdf:type owl:NamedIndividual ,
              :Pollutant ;
     rdfs:comment "An instance of class Pollutant" ;
     rdfs:label "PM1" .


###  http://www.semanticweb.org/radmehr/ontologies/2024/9/untitled-ontology-36/PM10
:PM10 rdf:type owl:NamedIndividual ,
               :Pollutant ;
      rdfs:comment "An instance of class Pollutant" ;
      rdfs:label "PM10" .


###  http://www.semanticweb.org/radmehr/ontologies/2024/9/untitled-ontology-36/PM2.5
:PM2.5 rdf:type owl:NamedIndividual ,
                :Pollutant ;
       rdfs:comment "An instance of class Pollutant" ;
       rdfs:label "PM2.5" .


###  http://www.semanticweb.org/radmehr/ontologies/2024/9/untitled-ontology-36/RelativeHumidity
:RelativeHumidity rdf:type owl:NamedIndividual ,
                           :Pollutant ;
                  rdfs:comment "An instance of class Pollutant" ;
                  rdfs:label "RelativeHumidity" .


###  http://www.semanticweb.org/radmehr/ontologies/2024/9/untitled-ontology-36/SO2
:SO2 rdf:type owl:NamedIndividual ,
              :Pollutant ;
     rdfs:label "SO2" .


###  http://www.semanticweb.org/radmehr/ontologies/2024/9/untitled-ontology-36/Temperature
:Temperature rdf:type owl:NamedIndividual ,
                      :Pollutant ;
             rdfs:label "Temperature" .


###  http://www.semanticweb.org/radmehr/ontologies/2024/9/untitled-ontology-36/UM003
:UM003 rdf:type owl:NamedIndividual ,
                :Pollutant ;
       rdfs:label "UM003" .


###  http://www.semanticweb.org/radmehr/ontologies/2024/9/untitled-ontology-36/c
:c rdf:type owl:NamedIndividual ,
            :Unit ;
   rdfs:comment "An instance of class Unit" ;
   rdfs:label "c" .


###  http://www.semanticweb.org/radmehr/ontologies/2024/9/untitled-ontology-36/microGramPerCubicMeter
:microGramPerCubicMeter rdf:type owl:NamedIndividual ,
                                 :Unit ;
                        rdfs:comment "An instance of class Unit" ;
                        rdfs:label "microGramPerCubicMeter" .


###  http://www.semanticweb.org/radmehr/ontologies/2024/9/untitled-ontology-36/particlesPerCubicCentimeter
:particlesPerCubicCentimeter rdf:type owl:NamedIndividual ,
                                      :Unit ;
                             rdfs:comment "An instance of class Unit" ;
                             rdfs:label "particlesPerCubicCentimeter" .


###  http://www.semanticweb.org/radmehr/ontologies/2024/9/untitled-ontology-36/percentage
:percentage rdf:type owl:NamedIndividual ,
                     :Unit ;
            rdfs:comment "An instance of class Unit" ;
            rdfs:label "percentage" .


###  Generated by the OWL API (version 4.5.29.2024-05-13T12:11:03Z) https://github.com/owlcs/owlapi
